sys-init/InitCSpace_SI.thy
@@ -58,6 +58,23 @@ lemma object_slot_spec2s:
    apply (simp_all add:object_slots_def update_slots_def)
   done
 
+lemma object_slots_frame_case_lift:
+  "object_slots
+         (case obj of Frame frame \<Rightarrow> Frame (f frame) | _ \<Rightarrow> g)
+         slot =
+   (case obj of Frame frame \<Rightarrow> None | _ \<Rightarrow> object_slots g slot)"
+by(cases obj; clarsimp simp add: object_slots_def)
+
+lemma object_slot_object_initialised_state:
+  "object_slots obj slot = object_slots obj' slot
+  \<Longrightarrow> object_slots (object_initialised_state t obj) slot =
+      object_slots (object_initialised_state t obj') slot"
+  apply (case_tac "has_slots obj")
+   apply (case_tac "has_slots obj'")
+    apply (clarsimp simp: object_initialised_state_def spec2s_def object_slots_frame_case_lift,
+            case_tac obj; case_tac obj'; clarsimp simp add: spec2s_def has_slots_def)+
+  done
+
 lemma irqhandler_cap_cap_irq [simp]:
   "is_irqhandler_cap cap \<Longrightarrow> IrqHandlerCap (cap_irq cap) = cap"
   by (clarsimp simp: cap_type_def cap_irq_def split: cdl_cap.splits)
@@ -228,7 +245,7 @@ lemma cnode_slot_half_initialised_not_original_slot:
                          object_slots_object_clean
                   split: option.splits)
    apply (cut_tac obj = "cnode_half spec obj_id spec_object" and
-                 obj' = spec_object and slot=slot and t=t in object_slot_spec2s)
+                 obj' = spec_object and slot=slot and t=t in object_slot_object_initialised_state)
     apply (erule object_slots_cnode_half)
    apply clarsimp
   apply (clarsimp simp: sep_map_s_def sep_map_general_def)
@@ -237,7 +254,7 @@ lemma cnode_slot_half_initialised_not_original_slot:
                         object_slots_object_clean
                  split: option.splits)
   apply (cut_tac obj = "cnode_half spec obj_id spec_object" and
-                obj' = spec_object and slot=slot and t=t in object_slot_spec2s)
+                obj' = spec_object and slot=slot and t=t in object_slot_object_initialised_state)
    apply (erule object_slots_cnode_half)
   apply clarsimp
   done
@@ -290,6 +307,30 @@ lemma object_slots_spec2s_cnode_half_object_default_state:
   apply clarsimp
   done
 
+lemma object_slots_object_initialised_state_cnode_half_object_default_state:
+  "\<lbrakk>well_formed spec; original_cap_at (obj_id, slot) spec;
+    cdl_objects spec obj_id = Some spec_object; is_cnode spec_object\<rbrakk>
+  \<Longrightarrow> object_slots (object_initialised_state t (cnode_half spec obj_id spec_object)) slot =
+      object_slots (object_default_state spec_object) slot"
+  apply (clarsimp simp: well_formed_def)
+  apply (erule_tac x=obj_id in allE)
+  apply (clarsimp split: option.splits)
+  apply (clarsimp simp: object_default_state_def2 is_cnode_def
+                 split: cdl_object.splits)
+  apply (rename_tac cnode)
+  apply (case_tac "slot < 2 ^ cdl_cnode_size_bits cnode")
+   apply (frule slots_empty_cnode1)
+   apply (frule_tac cnode=cnode and t=t in slots_spec2s_cnode_half1, assumption)
+    apply (clarsimp simp: object_slots_def dom_def empty_cnode_def empty_cap_map_def)
+    apply fastforce
+   apply (clarsimp simp: update_slots_def empty_cnode_def
+                         object_initialised_state_def cnode_half_def)
+  apply (frule slots_empty_cnode2)
+  apply (frule_tac cnode=cnode and t=t in slots_spec2s_cnode_half2, assumption)
+   apply (fastforce simp: object_slots_def dom_def empty_cnode_def empty_cap_map_def)
+  apply (clarsimp simp: update_slots_def object_initialised_state_def cnode_half_def)
+  done
+
 lemma cnode_slot_half_initialised_original_slot:
   "\<lbrakk>well_formed spec; original_cap_at (obj_id, slot) spec; cnode_at obj_id spec\<rbrakk>
   \<Longrightarrow> cnode_slot_half_initialised spec t obj_id slot
@@ -302,13 +343,13 @@ lemma cnode_slot_half_initialised_original_slot:
    apply (clarsimp simp: sep_map_s_def sep_map_general_def)
    apply (rule ext, clarsimp simp:object_to_sep_state_def
      object_project_def object_slots_object_clean)
-   apply (subst object_slots_spec2s_cnode_half_object_default_state)
+   apply (subst object_slots_object_initialised_state_cnode_half_object_default_state)
     apply simp+
     apply (clarsimp simp: object_at_def)+
   apply (clarsimp simp: sep_map_s_def sep_map_general_def)
   apply (rule ext)
   apply (clarsimp simp:object_to_sep_state_def object_project_def object_slots_object_clean)
-  apply (subst object_slots_spec2s_cnode_half_object_default_state, simp+)
+  apply (subst object_slots_object_initialised_state_cnode_half_object_default_state, simp+)
   apply (clarsimp split: option.splits)
   done
 
@@ -608,7 +649,7 @@ lemma mint_post:
   apply (frule_tac obj_id=dest_id in empty_cnode_object_size_bits, clarsimp)
   apply (cut_tac slot=slot in offset_slot, assumption, simp, simp)
   apply (subst sep_map_s_sep_map_c_eq [where cap="update_cap_object client_object_id spec_cap"])
-   apply (rule object_slots_spec2s, (clarsimp simp: opt_cap_def slots_of_def)+)
+   apply (rule object_slots_object_initialised_state, (clarsimp simp: opt_cap_def slots_of_def)+)
   apply (frule (2) well_formed_well_formed_cap, clarsimp simp: cap_has_object_def)
   apply (frule (2) well_formed_vm_cap_has_asid)
   apply (frule (1) well_formed_is_fake_vm_cap,
@@ -667,7 +708,7 @@ lemma mutate_post:
   apply (frule_tac obj_id=dest_id in empty_cnode_object_size_bits, clarsimp)
   apply (cut_tac slot=slot in offset_slot, assumption, simp, simp)
   apply (subst sep_map_s_sep_map_c_eq [where cap="update_cap_object client_object_id spec_cap"])
-   apply (rule object_slots_spec2s, (clarsimp simp: opt_cap_def slots_of_def)+)
+   apply (rule object_slots_object_initialised_state, (clarsimp simp: opt_cap_def slots_of_def)+)
   apply (frule (2) well_formed_well_formed_cap, clarsimp simp: cap_has_object_def)
   apply (frule (2) well_formed_vm_cap_has_asid)
   apply (frule (1) well_formed_is_fake_vm_cap,
@@ -724,7 +765,7 @@ lemma move_post:
   apply (frule_tac obj_id=dest_id in empty_cnode_object_size_bits, clarsimp)
   apply (cut_tac slot=slot in offset_slot, assumption, simp, simp)
   apply (subst sep_map_s_sep_map_c_eq [where cap="update_cap_object client_object_id spec_cap"])
-   apply (rule object_slots_spec2s, (clarsimp simp: opt_cap_def slots_of_def)+)
+   apply (rule object_slots_object_initialised_state, (clarsimp simp: opt_cap_def slots_of_def)+)
   apply (subst (asm) offset_slot', assumption)+
   apply (clarsimp simp: default_cap_cnode_dev)
   apply sep_solve
@@ -1100,6 +1141,16 @@ lemma irq_handler_cap_not_device[simp]:
  "is_irqhandler_cap y \<Longrightarrow> is_device_cap y = False"
  by (auto simp:is_device_cap_def split:cdl_cap.splits)
 
+lemma well_formed_original_irqhandler_cap_at:
+  "well_formed spec \<Longrightarrow> original_cap_at (obj_id, slot) spec
+   \<Longrightarrow> cap_at ((\<noteq>) NullCap) (obj_id, slot) spec
+   \<Longrightarrow> irqhandler_cap_at (obj_id, slot) spec"
+  apply (clarsimp simp: well_formed_def cap_at_def)
+  apply (frule opt_cap_dom_cdl_objects)
+  apply (drule_tac x=obj_id in spec)
+  apply (fastforce simp: well_formed_caps_def cap_at_def opt_cap_def slots_of_def)
+  done
+
 lemma init_cnode_slot_move_original_sep:
   "\<lbrakk>well_formed spec; cnode_at obj_id spec;
     original_cap_at (obj_id, slot) spec;
@@ -1129,34 +1180,14 @@ lemma init_cnode_slot_move_original_sep:
 
   (* Case: opt_cap (obj_id, slot) spec = None *)
   apply (case_tac "opt_cap (obj_id, slot) spec = None")
-   apply (clarsimp simp: init_cnode_slot_def assert_opt_def)
+   apply (clarsimp simp: cap_at_def)
   apply clarsimp
 
   (* Case: cap_at cap_has_object (obj_id, slot) spec *)
   apply (case_tac "cap_at cap_has_object (obj_id, slot) spec")
+   apply (frule (1) well_formed_original_irqhandler_cap_at)
+    apply (clarsimp simp: cap_at_def)
    apply (clarsimp simp: cap_at_def)
-   apply (rename_tac cap)
-   apply (frule (2) well_formed_cap_object)
-   apply (frule (2) well_formed_is_untyped_cap)
-   apply (clarsimp simp: init_cnode_slot_def)
-   apply (clarsimp simp: si_obj_cap_at_def si_obj_cap_at'_def cap_at_def
-                         si_spec_obj_null_cap_at_def si_spec_obj_null_cap_at'_def
-                         si_spec_irq_cap_at_def si_spec_irq_cap_at'_def
-                         si_spec_irq_null_cap_at_def si_spec_irq_null_cap_at'_def)
-   apply (wp seL4_CNode_Mutate_object_slot_initialised_sep seL4_CNode_Move_object_slot_initialised_cap_has_object_sep |
-          clarsimp)+
-   apply (intro impI conjI,simp_all add:)
-          apply (drule(1) well_formed_well_formed_cap[where obj_id = obj_id])
-            apply (simp add:opt_cap_def slots_of_def)
-           apply (simp add:cap_type_null)
-          apply simp
-         apply (metis cap_has_object_not_NullCap well_formed_cap_valid_src_cap well_formed_well_formed_cap')
-        apply (metis cap_has_object_not_NullCap well_formed_orig_ep_cap_is_default)
-       apply (simp add: ep_related_cap_def cap_type_def split:cdl_cap.splits)
-      apply (erule (3) well_formed_cnode_object_size_bits_eq)
-     apply (metis cap_has_object_NullCap well_formed_cap_has_object_has_type well_formed_well_formed_cap')
-    apply (metis cap_has_object_NullCap well_formed_cap_valid_src_cap well_formed_well_formed_cap')
-   apply (erule (3) well_formed_cnode_object_size_bits_eq)
 
   (* Case: cap_at is_irqhandler_cap (obj_id, slot) spec *)
   apply (frule (3) well_formed_cap_no_object_irqhandler_cap)
@@ -1173,12 +1204,12 @@ lemma init_cnode_slot_move_original_sep:
 lemma init_cnode_slot_move_not_original_inv:
   "\<lbrakk>\<not>original_cap_at (obj_id, slot) spec\<rbrakk>
   \<Longrightarrow> \<lbrace>P\<rbrace> init_cnode_slot spec orig_caps dup_caps irq_caps Move obj_id slot \<lbrace>\<lambda>_. P\<rbrace>"
-  apply (clarsimp simp: init_cnode_slot_def cap_at_def)
-  apply wp
-         apply (rule hoare_pre_cont)
-        apply (rule hoare_pre_cont)
-       apply clarsimp
-       apply wp+
+  apply (clarsimp simp: init_cnode_slot_def original_cap_at_def)
+  apply wpsimp
+                    apply (rule hoare_pre_cont)
+                   apply (rule hoare_pre_cont)
+                  apply clarsimp
+                  apply wp+
   apply clarsimp
   done
 
@@ -1339,10 +1370,15 @@ lemma init_cspace_move_sep:
   done
 
 lemma init_cnode_slot_copy_original_sep:
-  "\<lbrakk>original_cap_at (obj_id, slot) spec\<rbrakk>
+  "\<lbrakk>well_formed spec; cap_at (\<lambda>c. is_device_cap c = dev) (obj_id, slot) spec;
+    original_cap_at (obj_id, slot) spec\<rbrakk>
   \<Longrightarrow> \<lbrace>P\<rbrace> init_cnode_slot spec orig_caps dup_caps irq_caps Copy obj_id slot \<lbrace>\<lambda>_. P\<rbrace>"
-  apply (clarsimp simp: init_cnode_slot_def)
-  apply (wp|clarsimp)+
+  apply (case_tac "opt_cap (obj_id, slot) spec = Some NullCap")
+   apply (wpsimp simp: init_cnode_slot_def)
+  apply (frule (1) well_formed_original_irqhandler_cap_at)
+   apply (clarsimp simp: cap_at_def)
+  apply (clarsimp simp: init_cnode_slot_def cong: option.case_cong)
+  apply wpsimp
   done
 
 lemma ep_cap_default_cap:
@@ -1528,10 +1564,7 @@ lemma init_cnode_slot_copy_not_original_sep:
 
   (* Case: opt_cap (obj_id, slot) spec = None *)
   apply (case_tac "opt_cap (obj_id, slot) spec = None")
-   apply (clarsimp simp: init_cnode_slot_def)
-   apply (wp|clarsimp)+
-         apply (rule hoare_pre_cont)
-        apply (wp|clarsimp)+
+   apply (clarsimp simp: cap_at_def)
 
   (* Case: cap_at cap_has_object (obj_id, slot) spec *)
   apply (case_tac "cap_at cap_has_object (obj_id, slot) spec")
@@ -1560,6 +1593,7 @@ lemma init_cnode_slot_copy_not_original_sep:
        apply (rule_tac orig_cap=orig_cap and cap=cap and R=Ra
               in init_cnode_slot_copy_not_original_sep_helper, (simp|sep_solve)+)
   (* Case: cap_at is_irqhandler_cap (obj_id, slot) spec *)
+  apply clarsimp
   apply (frule (3) well_formed_cap_no_object_irqhandler_cap)
   apply (clarsimp simp: original_cap_at_def)
   done
@@ -1577,7 +1611,7 @@ lemma init_cnode_slot_copy_sep:
         si_cap_at t dup_caps spec dev obj_id \<and>*
         object_fields_empty spec t obj_id \<and>* si_objects \<and>* R\<guillemotright>\<rbrace>"
   apply (case_tac "original_cap_at (obj_id, slot) spec")
-   apply (wp init_cnode_slot_copy_original_sep, simp+)
+   apply (wp init_cnode_slot_copy_original_sep)
    apply (subst cnode_slot_half_initialised_original_slot, simp+)
   apply (subst cnode_slot_half_initialised_not_original_slot, assumption+)
   apply (wp init_cnode_slot_copy_not_original_sep, simp+)
@@ -1688,13 +1722,13 @@ lemma init_cspace_sep':
      si_objs_caps_at t orig_caps spec dev cnodes \<and>*
      si_spec_irqs_caps_at irq_caps spec cnodes \<and>*
      si_caps_at t dup_caps spec dev cnodes \<and>*
-     si_objects \<and>* R\<guillemotright> and K(
-     well_formed spec \<and>
-     set obj_ids = dom (cdl_objects spec) \<and>
-     distinct obj_ids \<and>
-     cnodes = {obj_id. cnode_at obj_id spec} \<and>
-     (\<forall>obj_id\<in> cnodes. \<forall>slot\<in> dom (slots_of obj_id spec). cap_at (\<lambda>c. is_device_cap c = dev) (obj_id,slot) spec))\<rbrace>
-   init_cspace spec orig_caps dup_caps irq_caps obj_ids
+     si_objects \<and>* R\<guillemotright> and
+    K (well_formed spec \<and>
+       set real_obj_ids = {obj_id. real_object_at obj_id spec} \<and>
+       distinct real_obj_ids \<and>
+       cnodes = {obj_id. cnode_at obj_id spec} \<and>
+       (\<forall>obj_id\<in> cnodes. \<forall>slot\<in> dom (slots_of obj_id spec). cap_at (\<lambda>c. is_device_cap c = dev) (obj_id,slot) spec))\<rbrace>
+   init_cspace spec orig_caps dup_caps irq_caps real_obj_ids
    \<lbrace>\<lambda>_.\<guillemotleft>objects_initialised spec t cnodes \<and>*
         si_spec_objs_null_caps_at t orig_caps spec cnodes \<and>*
         si_spec_irqs_null_caps_at irq_caps spec cnodes \<and>*
@@ -1735,6 +1769,10 @@ lemma set_take_add:
    set (take i zs) \<union> set (take j (drop i zs)) = set (take k zs)"
   by (metis set_append take_add)
 
+lemma distinct_take_drop_take:
+  "distinct xs \<Longrightarrow> set (take i (drop j xs)) \<inter> set (take j xs) = {}"
+  by (metis distinct_append distinct_take inf_commute take_add)
+
 lemma wellformed_no_dev:
   "well_formed spec \<Longrightarrow>(\<forall>obj_id. cnode_at obj_id spec \<longrightarrow>
                        (\<forall>slot\<in>dom (slots_of obj_id spec). cap_at (\<lambda>c. is_device_cap c = False) (obj_id, slot) spec))"
@@ -1748,18 +1786,19 @@ lemma init_cspace_sep:
      si_caps_at t orig_caps spec False {obj_id. real_object_at obj_id spec} \<and>*
      si_irq_caps_at irq_caps spec (used_irqs spec) \<and>*
      si_caps_at t dup_caps spec False {obj_id. cnode_or_tcb_at obj_id spec} \<and>*
-     si_objects \<and>* R\<guillemotright> and K(
-     well_formed spec \<and>
-     set obj_ids = dom (cdl_objects spec) \<and>
-     distinct obj_ids \<and>
-     distinct free_cptrs \<and>
-     orig_caps = map_of (zip [obj\<leftarrow>obj_ids. real_object_at obj spec] free_cptrs) \<and>
-     irq_caps = map_of (zip (used_irq_list spec) (drop (card {obj_id. real_object_at obj_id spec}) free_cptrs)) \<and>
-     length obj_ids \<le> length free_cptrs
-     )\<rbrace>
-   init_cspace spec orig_caps dup_caps irq_caps obj_ids
+     si_objects \<and>* R\<guillemotright> and
+    K (well_formed spec \<and>
+       set real_obj_ids = {obj_id. real_object_at obj_id spec} \<and>
+       distinct real_obj_ids \<and>
+       dom orig_caps = {obj_id. real_object_at obj_id spec} \<and>
+       bij_betw (the o orig_caps) {obj_id. real_object_at obj_id spec}
+                (set (list_take_region (length (filter (\<lambda>obj. real_object_at obj spec) real_obj_ids)) free_cptrs)) \<and>
+       irq_caps = map_of (zip_region (used_irq_list spec) (drop_region (card {obj_id. real_object_at obj_id spec}) free_cptrs)) \<and>
+       card (dom (cdl_objects spec)) \<le> length_region free_cptrs \<and>
+       valid_slot_region free_cptrs)\<rbrace>
+   init_cspace spec orig_caps dup_caps irq_caps real_obj_ids
    \<lbrace>\<lambda>_. \<guillemotleft>objects_initialised spec t {obj_id. cnode_at obj_id spec} \<and>*
-        (\<And>* cptr \<in> set (take (card (dom (cdl_objects spec))) free_cptrs). (si_cnode_id, unat cptr) \<mapsto>c NullCap) \<and>*
+        (\<And>* cptr \<in> set (list_take_region (card (dom (cdl_objects spec))) free_cptrs). (si_cnode_id, unat cptr) \<mapsto>c NullCap) \<and>*
          si_caps_at t dup_caps spec False {obj_id. cnode_or_tcb_at obj_id spec} \<and>*
          si_objects \<and>* R\<guillemotright>\<rbrace>"
   apply (rule hoare_gen_asm, clarsimp)
@@ -1767,8 +1806,8 @@ lemma init_cspace_sep:
   apply (frule well_formed_objects_real_or_irq)
   apply (frule well_formed_objects_only_real_or_irq)
   apply (frule well_formed_objects_card)
-  apply (insert distinct_card [where xs = obj_ids], clarsimp)
-  apply (insert distinct_card [where xs = "[obj\<leftarrow>obj_ids . real_object_at obj spec]", symmetric], clarsimp)
+  apply (insert distinct_card [where xs = real_obj_ids], clarsimp)
+  apply (insert distinct_card [where xs = "[obj\<leftarrow>real_obj_ids . real_object_at obj spec]", symmetric], clarsimp)
   apply (subst si_caps_at_conversion [where
                real_ids  = "{obj_id. real_object_at obj_id spec}" and
                cnode_ids = "{obj_id. cnode_at obj_id spec}", symmetric], simp+)
@@ -1777,23 +1816,24 @@ lemma init_cspace_sep:
                cnode_ids = "{obj_id. cnode_at obj_id spec}", symmetric], simp+)
   apply (subst si_caps_at_restrict [where P="\<lambda>ref. cnode_at ref spec" and
                                            xs="{obj_id. cnode_or_tcb_at obj_id spec}"])+
-  apply (wp sep_wp: init_cspace_sep'[where t=t and dev=False and cnodes="set [obj\<leftarrow>obj_ids. cnode_at obj spec]"])
+  apply (wp sep_wp: init_cspace_sep'[where t=t and dev=False and cnodes="set [obj\<leftarrow>real_obj_ids. cnode_at obj spec]"])
   apply (clarsimp simp: cnode_or_tcb_at_simps wellformed_no_dev)
   apply (frule wellformed_no_dev)
-   apply simp
+  apply simp
   apply sep_cancel+
   apply (sep_drule si_null_caps_at_simplified [where
-                       obj_ids = "[obj\<leftarrow>obj_ids. real_object_at obj spec]"
+                       obj_ids = real_obj_ids
                    and real_ids = "{obj_id. real_object_at obj_id spec}"
-                   and free_cptrs = free_cptrs], simp+)
+                   and free_cptrs = free_cptrs]; simp)
   apply (sep_drule si_irq_null_caps_at_simplified [where
-                       free_cptrs="drop (card {obj_id. real_object_at obj_id spec}) free_cptrs"
-                   and irqs="used_irq_list spec"], simp+)
+                       free_cptrs="drop_region (card {obj_id. real_object_at obj_id spec}) free_cptrs"
+                   and irqs="used_irq_list spec"]; simp)
   apply (subst (asm) sep.prod.union_disjoint [symmetric], simp+)
-   apply (metis (no_types) distinct_append distinct_take_strg inf_sup_aci(1) take_add)
+   apply (simp add: distinct_take_drop_take)
   apply (erule sep_map_set_conj_set_cong[THEN fun_cong, THEN iffD1, rotated])
   apply clarsimp
-  apply (subst Un_commute, subst set_take_add, (simp add: add.commute)+)
+  apply (subst Un_commute, subst set_take_add;
+         simp add: add.commute)
   done
 
 end
