sys-init/StaticDerivations_SI.thy
@@ -1,0 +1,227 @@
+(*
+ * Copyright 2021, Data61, CSIRO (ABN 41 687 119 230)
+ *
+ * SPDX-License-Identifier: GPL-2.0-only
+ *)
+
+theory StaticDerivations_SI
+imports
+  "DSpecProofs.Retype_DP"
+  Sep_Algebra.Extended_Separation_Algebra
+begin
+
+
+definition "spec_object_size spec ptr =
+  (let obj = (the (cdl_objects spec ptr)) in obj_bits_cdl (object_type obj) (object_size_bits obj))"
+
+definition "next_allocation spec previous current =
+   alignUp previous (spec_object_size spec current) + 2 ^ (spec_object_size spec current)"
+
+fun previous :: "'a \<Rightarrow> 'a list \<Rightarrow> 'a option"  where
+  "previous v [] = None" |
+  "previous v [x] = None" |
+  "previous v (x#y#xs) =  (if y = v then Some x else previous v (y#xs))"
+
+primrec allocate where
+   "allocate base_ptr spec [] = Map.empty" |
+   "allocate ptr spec (x#xs) = [x \<mapsto> ptr] + allocate (next_allocation spec ptr x ) spec xs"
+
+declare allocate.simps[simp del]
+
+definition "mapp g f = (\<lambda>x. map_option (g x) (f x))"
+
+definition "aligned_allocations spec base_ptr children =
+      mapp (\<lambda>ptr ptr'. alignUp ptr' (spec_object_size spec ptr)) (allocate base_ptr spec children)"
+
+lemma [simp]:
+  "mapp g (x + y) = mapp g x + mapp g y"
+  apply (intro ext iffI; clarsimp simp: mapp_def plus_fun_def plus_option_def split: option.splits)
+  done
+
+lemma [simp]:
+  "mapp g ([x \<mapsto> y]) = [x \<mapsto> g x y]"
+  apply (intro ext iffI; clarsimp simp: mapp_def plus_fun_def plus_option_def split: option.splits)
+  done
+
+lemma aligned_allocations_hd: "aligned_allocations spec ptr (a#list) a =
+  Some (alignUp ptr (spec_object_size spec a))"
+  apply (clarsimp simp: aligned_allocations_def allocate.simps)
+  apply (simp add: plus_fun_def plus_option_def)
+  done
+
+lemma mapp_app[simp]: "M x \<noteq> None \<Longrightarrow> (mapp f M) x = Some (f x (the (M x)))"
+  by (clarsimp simp: mapp_def)
+
+lemma [simp]: "distinct (x#xs) \<Longrightarrow>
+     ([x \<mapsto> v] + allocate y spec xs) x = Some v"
+  apply (induct xs; clarsimp simp: plus_fun_def plus_option_def)
+  done
+
+lemma [simp]: "distinct (x#xs) \<Longrightarrow>
+      ([x \<mapsto> v] + mapp g (allocate y spec xs)) x = Some v"
+  apply (induct xs; clarsimp simp: plus_fun_def plus_option_def)
+  done
+
+lemma [simp]: "allocate ptr spec (a # list) a = Some ptr"
+  apply (clarsimp simp: allocate.simps)
+  by (simp add: plus_fun_def plus_option_def)
+
+lemma not_in_previous: "x \<notin> set list \<Longrightarrow>
+   previous x list = None"
+  apply (induct list arbitrary: x; clarsimp)
+  by (metis list.set_intros(1) not_NilE previous.simps(2) previous.simps(3))
+
+lemma not_in_previous':"x \<notin> set list \<Longrightarrow> Some p = previous x (x # list) \<Longrightarrow> False"
+  apply (induct list arbitrary: x p; clarsimp)
+  by (simp add: not_in_previous)
+
+lemma in_tail_previous: "x \<in> set list \<Longrightarrow> previous x (a # list) \<noteq> None"
+  by (induct list arbitrary: a; clarsimp)
+
+lemma previous_in_head: "x \<in> set list \<Longrightarrow> the (previous x (a # list)) \<notin> set list
+        \<Longrightarrow> the (previous x (a # list)) = a"
+  by (induct list arbitrary: a; clarsimp)
+
+lemma previous_in_tail: "Some p = previous x (a # list) \<Longrightarrow> x \<in> set list"
+  by (induct list arbitrary: a; clarsimp split: if_splits)
+
+lemma in_right_map[simp]: "v \<noteq> x \<Longrightarrow> ([x \<mapsto> y] + ys) v = ys v"
+ by (clarsimp simp: plus_fun_def plus_option_def)
+
+lemma in_list_allocate: "x \<in> set list \<Longrightarrow> \<exists>z. allocate ptr spec (list) x = Some z"
+  apply (induct list arbitrary: ptr x)
+   apply (clarsimp)
+  apply (case_tac "x=a")
+   apply (clarsimp)
+  apply (drule meta_spec)
+  apply (drule_tac x=x in meta_spec)
+  apply (drule meta_mp)
+   apply (clarsimp)
+  apply (clarsimp)
+  apply (rule exI)
+  apply (clarsimp simp: allocate.simps(2))
+  apply (fastforce simp: in_right_map)
+  done
+
+lemma previous_in_list: "previous x list = Some y \<Longrightarrow> y \<in> set list"
+  apply (induct list arbitrary: y)
+   apply clarsimp+
+  apply (metis option.sel previous_in_head previous_in_tail)
+  done
+
+lemma distinct_previous_const:
+  "\<lbrakk>distinct (a#list); previous x list = Some y\<rbrakk> \<Longrightarrow> Some y = previous x (a # list)"
+  apply (induct list arbitrary: x y; clarsimp)
+  apply (metis previous_in_tail)
+  done
+
+lemma previous_in_allocate: "\<lbrakk>previous x list = Some y; distinct (a#list); x \<in> set list\<rbrakk>
+  \<Longrightarrow> \<exists>z. allocate ptr spec (a # list) y = Some z"
+  apply (drule (1) distinct_previous_const[rotated])
+  apply (drule sym)
+  apply (frule previous_in_list)
+  apply (erule in_list_allocate)
+  done
+
+lemma allocate_alignUp:
+  "distinct list \<Longrightarrow>
+       x \<in> set list \<Longrightarrow>
+       (aligned_allocations spec (ptr :: machine_word) list) x =
+   Some (alignUp (the (allocate (ptr :: machine_word) spec list x))
+  (obj_bits_cdl (object_type (the (cdl_objects spec x))) (object_size_bits (the (cdl_objects spec x)))))"
+  supply allocate.simps[simp]
+  apply (induct list arbitrary: ptr; clarsimp)
+  apply (clarsimp simp: aligned_allocations_def)
+  apply (elim disjE; clarsimp)
+   apply (clarsimp simp: spec_object_size_def Let_unfold)
+  apply (subst in_right_map; clarsimp)
+  apply (subst in_right_map; clarsimp)
+  done
+
+lemma some_previous: "\<lbrakk>a \<notin> set list; Some a = previous x (a#list)\<rbrakk> \<Longrightarrow> x = hd list"
+  apply (induct list arbitrary: x a; clarsimp)
+  apply (metis Some_to_the empty_iff list.exhaust_sel list.set(1)
+               not_in_previous option.distinct(1) previous.simps(3) set_ConsD)
+  done
+
+lemma previous_cons[simp]: "a \<notin> set list \<Longrightarrow> p \<noteq> a \<Longrightarrow>
+     Some p = previous x (a # list) \<Longrightarrow> previous x (a # list) = previous x list"
+  by (induct list; clarsimp)
+
+lemma allocate_previous: "\<lbrakk>distinct list; x \<in> set list; Some p = previous x list\<rbrakk> \<Longrightarrow>
+       (allocate ptr spec  list) x = Some (next_allocation spec (the (allocate ptr spec list p)) p)"
+  apply (subgoal_tac "p \<in> set list")
+   supply allocate.simps[simp]
+   apply (induct list arbitrary: p ptr)
+    apply (clarsimp simp: aligned_allocations_def)
+   apply (frule previous_in_tail, clarsimp)
+   apply (elim disjE; clarsimp?)
+    apply (frule some_previous)
+     apply (clarsimp, rule refl)
+    apply (subst in_right_map)
+     apply clarsimp
+    apply (case_tac "list")
+     apply fastforce+
+   apply (subst in_right_map)
+    apply clarsimp
+   apply (frule previous_in_tail, clarsimp)
+   apply (drule_tac x=p in meta_spec)
+   apply (drule_tac x="(next_allocation spec ptr a)" in meta_spec)
+   apply clarsimp
+   apply (drule meta_mp)
+    apply clarsimp
+    apply (case_tac list)
+     apply clarsimp+
+   apply (subst in_right_map; clarsimp)
+  apply (induct list arbitrary: p; clarsimp)
+  apply (metis previous_cons previous_in_tail)
+  done
+
+lemma aligned_allocate_previous:
+  "\<lbrakk>distinct list; x \<in> set list; Some p = previous x list \<rbrakk> \<Longrightarrow>
+    (aligned_allocations spec  ptr  list) x =
+       Some (alignUp ((next_allocation spec (the (allocate (ptr :: machine_word) spec list p)) p))
+         (obj_bits_cdl (object_type (the (cdl_objects spec x))) (object_size_bits (the (cdl_objects spec x)))))"
+  apply (unfold aligned_allocations_def mapp_def)
+  apply (subst arg_cong[OF allocate_previous,
+                        where f="map_option (\<lambda>ptr'. alignUp ptr' (spec_object_size spec x))"])
+     apply (fastforce)+
+  apply (metis option.simps(9) spec_object_size_def)
+  done
+
+abbreviation cptr_of ::
+  "(cdl_cptr \<times> bi_untyped_desc \<times> cdl_cap) option \<Rightarrow> cdl_cptr"
+  where
+  "cptr_of \<equiv> \<lambda>x. fst (the x)"
+
+abbreviation cap_of ::
+  "(cdl_cptr \<times> bi_untyped_desc \<times> cdl_cap) option \<Rightarrow> cdl_cap"
+  where
+  "cap_of \<equiv> \<lambda>x. snd (snd (the x))"
+
+definition valid_derivations where
+  "valid_derivations spec untyped_derivations untyped_map \<equiv>
+    distinct (map fst untyped_derivations) \<and>
+    distinct_sets (map (set o snd) untyped_derivations) \<and>
+    (\<forall>family\<in>(set untyped_derivations).
+      let parent      = fst family;
+          parent_cap  = cap_of (untyped_map parent);
+          start       = Min (available_range (parent_cap));
+          children    = snd family
+      in
+        distinct children \<and>
+        (\<forall>child\<in>(set children).
+          let spec_child = the (cdl_objects spec child);
+              child_size = spec_object_size spec child
+          in
+            cdl_objects spec child \<noteq> None \<and>
+            object_type spec_child \<noteq> UntypedType \<and>
+            object_size_bits spec_child < 2 ^ word_bits \<and>
+            start \<le> start + 2 ^ child_size \<and>
+            child_size < word_size \<and>
+            is_aligned start child_size \<and>
+            start \<le> the (aligned_allocations spec start children child) + 2 ^ child_size \<and>
+            (previous child children \<noteq> None \<longrightarrow> start < the (allocate start spec children child)) \<and>
+            the (allocate start spec children child) \<in> available_range (parent_cap)))"
+
+end
